theories/AlmostStlc/MrecMonad.v
@@ -25,40 +25,177 @@ Require Import Program.Tactics.
 
 Require Import ITree.Basics.Basics.
 
+Require Export TypedVar.
+
+From Equations Require Import Equations Signature.
 
 Variant void : Set := .
 Global Instance voidEncodedType : EncodedType void := fun v => match v with end.
 
+Notation "a && b" := (existT _ a b).
 
-(* interp_mtree *)
+Notation mrec_ctx := (list {T : Type & EncodedType T}).
 
-(* could extend to have arbitrary constraints on E, could allow E to include other events*)
-(* universe inconsistenty traces back to here, for now could specialize E to void, perhaps,
-   this whole mtree idea was a holdover from when you had more complicated mfix effects *)
-Definition mtree (D : Type) `{EncodedType D} (A : Type) : Type@{entree_u}:= 
-   entree (D + void) A.
-
-Global Instance mtree_monad D `{EncodedType D} : Monad (mtree D) := Monad_entree.
-
-
-Definition call {D} `{EncodedType D} (d : D) : mtree D (encodes d) := trigger d.
-
-CoFixpoint interp_mtree' {D D' R} `{EncodedType D} `{EncodedType D'}
-           (bodies : forall (d : D), entree (D + void) (encodes d)) (ot : entree' (D + void) R ) : 
-  entree (D' + void) R :=
-  match ot with
-  | RetF r => Ret r
-  | TauF t => Tau (interp_mtree' bodies (observe t))
-  | VisF (inl d) k => 
-      Tau (interp_mtree' bodies (observe (EnTree.bind (bodies d) k ) ) )
-  | VisF (inr v) k => Vis (@inr D' void v) (fun x => interp_mtree' bodies (observe (k x)))
+Fixpoint denote_mrec_ctx (MR : mrec_ctx) : Type@{entree_u} :=
+  match MR with
+  | nil => void
+  | cons (T && _) MR => T + denote_mrec_ctx MR 
   end.
 
-Definition interp_mtree {D D' R} `{EncodedType D} `{EncodedType D'}
-           (bodies : forall (d : D), entree (D + void) (encodes d)) (t : entree (D + void) R) :
-  entree (D' + void) R := interp_mtree' bodies (observe t).
+Fixpoint encoded_mrec_ctx (MR : mrec_ctx) : EncodedType (denote_mrec_ctx MR) :=
+  match MR with
+  | nil => fun _ => void
+  | cons (T1 && encodes) MR =>
+      fun x => match x with
+            | inl y => encodes y
+            | inr y => encoded_mrec_ctx MR y
+            end
+  end.
+
+Global Instance encoded_mrec_ctx_instance MR : EncodedType (denote_mrec_ctx MR) := encoded_mrec_ctx MR.
+
+Definition mtree MR A : Type@{entree_u} :=
+  entree (denote_mrec_ctx MR) A.
+Notation mtree' MR A := (entree' (denote_mrec_ctx MR) A).
+
+Equations bring_to_front {A : Type} (MR : mrec_ctx) (In : Type) (Out : EncodedType In)
+          (x : var (In && Out) MR)
+          (e : denote_mrec_ctx MR)
+          (k : encodes e -> A)
+  : {i : In & encodes i -> A} + {e : denote_mrec_ctx (remove (In && Out) MR x) & encodes e -> A}   :=
+  bring_to_front ((In && Out) :: MR) In Out (VarZ _ MR) (inl i) k :=
+    inl (i && k);
+  bring_to_front ((In && Out) :: MR) In Out (VarZ _ MR) (inr e) k := inr (e && k);
+  bring_to_front ((T1 && T2) :: MR) In Out (VarS _ _ MR y) (inl i) k := inr ((inl i) && k);
+  bring_to_front ((T1 && T2) :: MR) In Out (VarS _ _ MR y) (inr e) k :=
+    match bring_to_front MR In Out y e k with
+    | inl (i && k ) => inl (i && k)
+    | inr (e && k) => inr ((inr e) && k )
+    end.
+
+Lemma bring_to_front_k_inl_jmeq : forall A MR In Out (x : var (In && Out) MR) (e : denote_mrec_ctx MR) (k : encodes e -> A) i k',
+    bring_to_front MR In Out x e k = inl (i && k') -> k ~= k'.
+Proof.
+  intros A R In Out x. dependent induction x.
+  - intros [ | ]; intros; try discriminate.
+    simp bring_to_front in H. injection H. intros. subst. apply inj_pair2 in H0. subst. auto.
+  - destruct b. cbn. intros [ | ]; try discriminate.
+    simp bring_to_front. intros. eapply IHx; eauto. Unshelve. all : auto.
+    simp bring_to_front in H. destruct (bring_to_front l In Out x d k) as [ | ]; destruct s; try discriminate.
+    injection H. intros. subst. apply inj_pair2 in H0. subst. auto.
+Qed.
 
 
-(* consider a more complicated mtree monad where you have a list of event types 
-   and interp_mtree requires an index and can an event at that index 
-*)
+Lemma bring_to_front_k_inr_jmeq : forall A MR In Out (x : var (In && Out) MR) (e : denote_mrec_ctx MR) (k : encodes e -> A) e' k',
+    bring_to_front MR In Out x e k = inr (e' && k') -> k ~= k'.
+Proof.
+  intros A R In Out x. dependent induction x.
+  - intros [ | ]; intros; try discriminate. simp bring_to_front in H.
+    cbn in *.  setoid_rewrite bring_to_front_equation_3 in H.
+    injection H. intros. subst. dependent destruction H0. auto.
+  - destruct b. cbn in *. intros [ | ]; intros; try discriminate.
+    + intros. simp bring_to_front in H. injection H. intros. subst.
+      match goal with H : inr ?a1 = inr ?a2 |- _ => remember a1 as ek1; remember a2 as ek2; 
+                                                  assert (ek1 = ek2) end.
+      injection H. intros; auto.
+      rewrite Heqek1 in H0. rewrite Heqek2 in H0.
+      apply inj_pair2 in H0. subst. auto.
+    + cbn in H. simp remove in *. simp bring_to_front in H.
+      destruct (bring_to_front l In Out x d k ) as [ | ] eqn :Heq; destruct s; try discriminate.
+      injection H. intros. subst. eapply IHx; eauto.
+      rewrite Heq.
+      match goal with H : inr ?a1 = inr ?a2 |- _ => remember a1 as ek1; remember a2 as ek2; 
+                                                  assert (ek1 = ek2) end.
+      { injection H. auto. }
+      clear H. rewrite Heqek1 in H0. rewrite Heqek2 in H0.
+      apply inj_pair2 in H0. subst. auto.
+Qed.
+
+Section interp_mtree.
+Context (MR : mrec_ctx) (In : Type) (Out : EncodedType In) (x : var (In && Out) MR).
+
+Context (body : forall i : In, mtree MR (encodes i)).
+
+CoFixpoint interp_mtree' {A} (om : mtree' MR A) : mtree (remove (In && Out) MR x) A :=
+  match om with
+  | RetF r => Ret r
+  | TauF t => Tau (interp_mtree' (observe t))
+  | VisF e k => 
+      match bring_to_front MR In Out x e k with
+      | inl (i && k') => Tau (interp_mtree' (observe (EnTree.bind (body i) k')))
+      | inr (e' && k') => Vis e' (fun x  => interp_mtree' (observe (k' x)) )
+      end
+  end.
+
+Definition interp_mtree {A} (m : mtree MR A) : mtree (remove (In && Out) MR x) A :=
+  interp_mtree' (observe m).
+
+End interp_mtree.
+
+
+Definition handler (D1 D2 : Type) `{EncodedType D1} `{EncodedType D2}  :=
+  forall (d : D1), {d' : D2 & encodes d' -> encodes d}.
+
+CoFixpoint mapE' {D1 D2 R} `{EncodedType D1} `{EncodedType D2} (h : handler D1 D2)
+           (ot : entree' D1 R) : entree D2 R :=
+  match ot with
+  | RetF r => Ret r
+  | TauF t => Tau (mapE' h (observe t))
+  | VisF d k => let '(d' && f) := h d in
+               Vis d' (fun x => mapE' h (observe (k (f x))))
+  end.
+
+Definition mapE {D1 D2 R} `{EncodedType D1} `{EncodedType D2} (h : handler D1 D2)
+           (t : entree D1 R) : entree D2 R :=
+  mapE' h (observe t).
+
+(* another function that builds very slowly *)
+Equations perm_handler (MR1 MR2 : mrec_ctx) (Hperm : perm MR1 MR2)
+          (d : denote_mrec_ctx MR1) : {d' : denote_mrec_ctx MR2 & encodes d' -> encodes d} :=
+  perm_handler nil nil perm_nil v := match v : void with end;
+  perm_handler ((T1 && T2) :: MR1) ((T1 && T2) :: MR2) (perm_skip _ MR1 MR2 Hperm)
+               (inl i) := (inl i && id);
+  perm_handler ((T1 && T2) :: MR1) ((T1 && T2) :: MR2) (perm_skip _ MR1 MR2 Hperm)
+               (inr d) := let '(d' && f) := perm_handler MR1 MR2 Hperm d in
+                          (inr d' && f);
+  perm_handler _ _ (perm_swap _ _ _ _ Hperm)
+               (inl i) := (inr (inl i) && id);
+  perm_handler _ _ (perm_swap _ _ _ _ Hperm)
+               (inr (inl i)) := (inl i && id);
+  perm_handler _ _ (perm_swap _ _ MR1 MR2 Hperm)
+               (inr (inr d)) := let '(d' && f) := perm_handler MR1 MR2 Hperm d in
+                                (inr (inr d') && f );
+  perm_handler MR1 MR3 (perm_trans MR1 MR2 MR3 Hp12 Hp23) d1 :=
+    let '(d2 && f12) := perm_handler MR1 MR2 Hp12 d1 in
+    let '(d3 && f23) := perm_handler MR2 MR3 Hp23 d2 in
+    (d3 && (fun x => f12 (f23 x) )).
+
+Definition map_perm MR1 MR2 (Hperm : perm MR1 MR2) {A} (m : mtree MR1 A) :
+  mtree MR2 A :=
+  mapE (perm_handler MR1 MR2 Hperm) m.
+
+Equations concat_handler (MR1 MR2 : mrec_ctx) (d : denote_mrec_ctx MR2) :
+          {d' : denote_mrec_ctx (MR1 ++ MR2) & encodes d' -> encodes d } :=
+  concat_handler nil MR2 d := (d && id);
+  concat_handler ((T1 && T2) :: MR1 ) MR2 d :=
+    let '(d' && f) := concat_handler MR1 MR2 d in
+    (inr d' && f).
+
+Definition map_concat MR1 MR2 {A} (m : mtree MR2 A) : mtree (MR1 ++ MR2) A :=
+  mapE (concat_handler MR1 MR2) m.
+
+
+Global Instance Monad_mtree MR : (Monad (mtree MR)) := Monad_entree.
+
+Equations call {MR T1} {T2 : EncodedType T1} (x : var (T1 && T2) MR) (v : T1) : 
+  {d : denote_mrec_ctx MR & encodes d -> encodes v} :=
+  call (VarZ _ _) v := (inl v && id);
+  call (VarS _ (_ && _) _ y) v := let '(d && f) := call y v in
+                           (inr d && f).
+
+Definition callm {MR T1} {T2 : EncodedType T1} (x : var (T1 && T2) MR) (v : T1) : 
+  mtree MR (encodes v) :=
+  let '(d && f) := call x v in
+  bind (EnTree.trigger d) (fun x => Ret (f x)).
+
+                        
