theories/AlmostStlc/Syntax.v
@@ -1,40 +1,36 @@
-
-
-Inductive var {T : Type} : T -> list T -> Type := 
-  | VarZ (x : T) l : var x (x :: l)
-  | VarS (x y : T) l : var x l -> var x (y :: l).
-
+Require Export TypedVar.
 
 Inductive type : Type :=
   | Nat : type
   | List : type -> type
-                   (* should really be a nonempty list *)
-  | Arrow : type -> list (type * type) -> type -> type
+  | Arrow : type -> (list (list (type * type))) -> type -> type
 .
 Notation ctx := (list type).
-Notation rec_ctx := (list (type * type))%type.
+Notation call_frame := (list (type * type)).
+Notation mfix_ctx := (list call_frame).
 
 
 
 (*TODO : add some basic natural number operations *)
-Inductive term : type -> ctx -> rec_ctx -> Type := 
-  | term_const (n : nat) Γ R : term Nat Γ R
-  | term_nil t Γ R : term (List t) Γ R
-  | term_cons t Γ R (head : term t Γ R) (tail : term (List t) Γ R) : term (List t) Γ R
-  | term_var t Γ R (x : var t Γ) : term t Γ R
+Inductive term : type -> ctx -> mfix_ctx -> Type := 
+  | term_const (n : nat) Γ MR : term Nat Γ MR
+  | term_nil t Γ MR : term (List t) Γ MR
+  | term_cons t Γ MR (head : term t Γ MR) (tail : term (List t) Γ MR) : term (List t) Γ MR
+  | term_var t Γ MR (x : var t Γ) : term t Γ MR
 
-  | term_match_nat t Γ R (en : term Nat Γ R) (eZ : term t Γ R) (eS : term t (Nat :: Γ) R ) : term t Γ R
-  | term_match_list t1 t2 Γ R (el : term (List t1) Γ R ) (enil : term t2 Γ R) (econs : term t2 (t1 :: List t1 :: Γ) R) : term t2 Γ R
+  | term_match_nat t Γ MR (en : term Nat Γ MR) (eZ : term t Γ MR) (eS : term t (Nat :: Γ) MR ) : term t Γ MR
+  | term_match_list t1 t2 Γ MR (el : term (List t1) Γ MR ) (enil : term t2 Γ MR) (econs : term t2 (t1 :: List t1 :: Γ) MR) : term t2 Γ MR
   (* might be some subtleties in the application rule you are not sufficiently considering *)
-  | term_app t1 t2 Γ R (e1 : term (Arrow t1 R t2) Γ R) (e2 : term t1 Γ R) : term t2 Γ R
+  | term_app t1 t2 Γ MR (e1 : term (Arrow t1 MR t2) Γ MR) (e2 : term t1 Γ MR) : term t2 Γ MR
   (* same here *)
-  | term_abs t1 t2 Γ R R' (e : term t2 (t1 :: Γ) R') : term (Arrow t1 R' t2) Γ R
-  | term_call t1 t2 Γ R (x : var (t1,t2) R) (arg : term t1 Γ R) : term t2 Γ R
-  (* this is the most novel part so be very careful *)
-  | term_mfix t Γ R R' (bodies : mfix_bodies Γ R R) (e : term t Γ R) : term t Γ R'
+  | term_abs t1 t2 Γ MR MR' (e : term t2 (t1 :: Γ) MR') : term (Arrow t1 MR' t2) Γ MR
+  | term_perm t Γ MR1 MR2 (Hperm : perm MR1 MR2) (e : term t Γ MR1) : term t Γ MR2
+  | term_lift t Γ MR1 MR2 (e : term t Γ MR2) : term t Γ (MR1 ++ MR2)
+  | term_call t1 t2 Γ MR R (xR : var R MR) (x : var (t1,t2) R) (arg : term t1 Γ MR) : term t2 Γ MR
+  | term_mfix t Γ R MR (x : var R MR) (bodies : mfix_bodies Γ MR R) (e : term t Γ MR) : term t Γ (remove R MR x)
 
-
-with mfix_bodies : ctx -> rec_ctx -> rec_ctx -> Type := 
-  | mfix_bodies_nil Γ R : mfix_bodies Γ R nil
-  | mfix_bodies_cons Γ R t1 t2 R' (body : term t2 (t1 :: Γ) R) (bodies : mfix_bodies Γ R R') : mfix_bodies Γ R ((t1,t2) :: R')
+with mfix_bodies : ctx -> mfix_ctx -> call_frame -> Type :=
+  | mfix_bodies_nil Γ MR : mfix_bodies Γ MR nil
+  | mfix_bodies_cons Γ MR t1 t2 R' (body : term t2 (t1 :: Γ) MR) (bodies : mfix_bodies Γ MR R') :
+    mfix_bodies Γ MR ((t1,t2) :: R')
 .
